Cleanup UGraph, no "GC set" anymore

common/theories/uGraph.v
@@ -1,5 +1,5 @@
 (* Distributed under the terms of the MIT license. *)
-From Stdlib Require Import ssreflect ssrbool OrderedTypeAlt MSetAVL MSetFacts MSetProperties MSetDecide Morphisms.
+From Stdlib Require Import ssreflect ssrbool ssrfun OrderedTypeAlt MSetAVL MSetFacts MSetProperties MSetDecide Morphisms.
 From MetaRocq.Utils Require Import utils.
 From MetaRocq.Common Require Import config UnivConstraintType Universes UnivLoopChecking.
 From Equations.Prop Require Import DepElim.
@@ -11,7 +11,7 @@ Definition universe_model := UnivLoopChecking.univ_model.
 Definition init_model : universe_model := UnivLoopChecking.init_model.
 
 Definition uctx_invariants (uctx : ContextSet.t)
-  := UnivConstraintSet.For_all (declared_univ_cstr_levels uctx.1) uctx.2.
+  := UnivLoopChecking.declared_univ_cstrs_levels uctx.1 uctx.2.
 
 Definition global_uctx_invariants (uctx : ContextSet.t)
   := ~ LevelSet.In Level.lzero uctx.1 /\ uctx_invariants uctx.
@@ -26,7 +26,11 @@ push_uctx g uctx with UnivLoopChecking.declare_levels g uctx.1 :=
 
 Instance declared_univ_cstrs_levels_proper : Proper (LevelSet.Equal ==> UnivConstraintSet.Equal ==> iff)
   declared_univ_cstrs_levels.
-Proof. Admitted.
+Proof.
+  move=> ?? e ?? e'.
+  rewrite /declared_univ_cstrs_levels.
+  rewrite e'. rewrite /UnivConstraintSet.For_all /declared_univ_cstr_levels.
+Admitted.
 
 Definition push_uctx_precond g uctx :=
   let allcstrs := UnivConstraintSet.union uctx.2 (UnivConstraintSet.union (init_constraints_of_levels uctx.1) (constraints g)) in
@@ -67,6 +71,14 @@ Proof.
   - left. have := declare_levels_spec g uctx.1.
     now rewrite Heq.
 Qed.
+
+End Push.
+
+Import UnivLoopChecking.
+
+Definition is_model_of_uctx m uctx :=
+  levels m =_lset LevelSet.union uctx.1 (LevelSet.singleton Universes.Level.lzero) /\
+  constraints m =_ucset UnivConstraintSet.union uctx.2 (init_constraints_of_levels uctx.1).
 
 (** ** Check of consistency ** *)
 
@@ -123,6 +135,9 @@ Section CheckLeqProcedure.
 
   Definition check_constraint_gen (c : UnivConstraint.t) :=
     ~~ check_univs || check_cstr c.
+
+  Definition check_constraints_gen (c : UnivConstraintSet.t) :=
+    ~~ check_univs || UnivConstraintSet.for_all check_cstr c.
 
   Definition eqb_univ_instance_gen (u1 u2 : Instance.t) : bool :=
     forallb2 check_eqb_universe_gen u1 u2.
@@ -227,7 +242,10 @@ Section CheckLeq.
     interp_cstrs v (UnivConstraintSet.union cstrs cstrs') <->
     interp_cstrs v cstrs /\ interp_cstrs v cstrs'.
   Proof.
-  Admitted.
+    rewrite /interp_cstrs /UnivConstraintSet.For_all.
+    setoid_rewrite UnivConstraintSet.union_spec.
+    firstorder.
+  Qed.
 
   Lemma interp_nes_val (v : valuation) (u : Universe.t) :
     Universe.interp_nes (val v) u = Universes.val v u.
@@ -252,7 +270,6 @@ Section CheckLeq.
         rewrite !interp_nes_val. cbn. lia.
       * rewrite !interp_nes_val. cbn. constructor. lia.
   Qed.
-
 
   Lemma satisfies0_interp_cstr_inv V (v : Level.t -> nat) c :
     wf_valuation V v ->
@@ -297,61 +314,143 @@ Section CheckLeq.
     now exists cs; split => //.
   Qed.
 
+  Definition wf_zero_valuation V v :=
+    forall l, LevelSet.In l V ->
+    let zero := LS.Level.zero in
+    if l == zero then True
+    else if LS.Level.is_global l then v l > v zero
+    else v l >= v zero.
+
+  Lemma wf_valuation_zero V v :
+    wf_valuation V v ->
+    v Level.lzero = 0 ->
+    wf_zero_valuation V v.
+  Proof.
+    rewrite /wf_valuation /wf_zero_valuation.
+    move=> hl l hz /hl. destruct eqb => //.
+    now rewrite l.
+  Qed.
+
+  Lemma wf_zero_valuation_init v :
+    interp_cstrs v (init_constraints_of_levels uctx.1) ->
+    wf_zero_valuation uctx.1 v.
+  Proof.
+    intros hi l hin. unfold LS.Level.zero.
+    change (l == Level.lzero) with (eqb l Level.lzero).
+    destruct (eqb_spec l Level.lzero) => //.
+    destruct LS.Level.is_global eqn:isg.
+    - specialize (hi (U1, Le, Universe.singleton (l,0))).
+      forward hi.
+      eapply init_constraints_of_levels_spec. tea.
+      rewrite /init_constraint_of_level. destruct l => //.
+      destruct l as [|g|i]=> //.
+      cbn -[Pos.to_nat] in hi.
+      destruct (v (Level.level g)) eqn:hv => //. noconf hi. lia.
+    - specialize (hi (U0, Le, Universe.singleton (l,0))).
+      forward hi.
+      eapply init_constraints_of_levels_spec. tea.
+      rewrite /init_constraint_of_level. destruct l => //.
+      destruct l as [|g|i]=> //.
+      cbn -[Pos.to_nat] in hi. lia.
+  Qed.
+
   Definition shift_valuation (v : Level.t -> nat) : Level.t -> nat :=
     fun l => v l - v Level.lzero.
 
-  Lemma wf_shift_valuation v :
-    interp_cstrs v (init_constraints_of_levels uctx.1) ->
-    wf_valuation uctx.1 (shift_valuation v).
+  Lemma wf_shift_valuation V v :
+    wf_zero_valuation V v ->
+    wf_valuation V (shift_valuation v).
   Proof.
-    intros hi l hin. unfold LS.Level.zero.
+    move=> wfv l /wfv. cbn. unfold LS.Level.zero.
     change (l == Level.lzero) with (eqb l Level.lzero).
     have he : shift_valuation v Level.lzero = 0.
     rewrite /shift_valuation //. lia.
     destruct (eqb_spec l Level.lzero).
     - now subst l.
-    - destruct LS.Level.is_global eqn:isg.
-      unfold shift_valuation.
-      specialize (hi (U1, Le, Universe.singleton (l,0))).
-      forward hi.
-      eapply init_constraints_of_levels_spec; tea.
-      rewrite /init_constraint_of_level. destruct l => //.
-      destruct l as [|g|i]=> //.
-      cbn -[Pos.to_nat] in hi.
-      destruct (v (Level.level g)) eqn:hv => //. noconf hi. lia.
-      lia.
+    - destruct LS.Level.is_global eqn:isg; unfold shift_valuation; lia.
   Qed.
-  Lemma interp_nes_shift V (v : Level.t -> nat) (u : Universe.t) :
-    interp_cstrs v (init_constraints_of_levels uctx.1) ->
-    wf_valuation V (shift_valuation v) ->
-    LevelSet.Subset (Universe.levels u) V ->
-    Universe.interp_nes v u - v Level.lzero = Universe.interp_nes (shift_valuation v) u.
-  Proof.
-    move: u. refine (Universe.interp_nes_elim v (fun u i => _ -> _ -> _ -> i - v Level.lzero = Universe.interp_nes (shift_valuation v) u) _ _ _).
-    - intros [l k] whi wf hsub. rewrite /Universe.interp_expr //=
-        Universe.interp_nes_singleton /val; cbn in *.
 
-      specialize (wf l). forward wf. admit.
+  Lemma wf_valuation_neq V v :
+    wf_zero_valuation V v ->
+    forall l, LevelSet.In l V -> v l >= v LS.Level.zero.
+  Proof.
+    intros wfv l hin.
+    move: (wfv l hin).
+    unfold LS.Level.zero in *.
+    change (l == Level.lzero) with (eqb l Level.lzero).
+    destruct (eqb_spec l Level.lzero) => //=. subst. lia.
+    destruct l; cbn; try congruence; lia.
+  Qed.
+
+  Lemma interp_nes_shift {V} {v : Level.t -> nat} {u : Universe.t} :
+    wf_zero_valuation V v ->
+    LevelSet.Subset (Universe.levels u) V ->
+    Universe.interp_nes (shift_valuation v) u =
+    Universe.interp_nes v u - v Level.lzero /\ Universe.interp_nes v u >= v Level.lzero.
+  Proof.
+    move: u. refine (Universe.interp_nes_elim v (fun u i => _ -> _ ->
+      Universe.interp_nes (shift_valuation v) u = i - v Level.lzero /\ i >= v Level.lzero) _ _ _).
+    - intros [l k] wf hsub. rewrite /Universe.interp_expr //=
+        Universe.interp_nes_singleton /val; cbn in *.
+      specialize (wf l). forward wf.
+      { apply hsub. unfold flip; cbn. lsets. }
       rewrite /shift_valuation in wf |- *.
       move: wf. unfold LS.Level.zero.
       change (l == Level.lzero) with (eqb l Level.lzero).
       destruct (eqb_spec l Level.lzero) => //=. subst. lia.
       destruct l; cbn. congruence. lia.
-      cbn. intros.
-    - move=>[l k] u k' ih hnin.
-      cbn. rewrite val_add //=. cbn. subst k'. cbn.
-      reflexivity.
-  Qed. *)
-  Lemma interp_cstr_shift V v c :
-    wf_valuation V (shift_valuation v) ->
+      cbn. intros. lia.
+    - move=>[l k] u k' ih hnin wfv hsub.
+      specialize (ih wfv). cbn. erewrite Universe.interp_nes_add.
+      forward ih. setoid_rewrite <- hsub.
+      rewrite Universe.levels_add. lsets.
+      destruct ih as [ih ih']. rewrite ih.
+      move: (wf_valuation_neq _ _ wfv l) => /fwd.
+      apply hsub. rewrite Universe.levels_add //=. lsets.
+      rewrite /Universe.interp_expr //= /shift_valuation //=.
+      unfold LS.Level.zero; split; [lia|]. lia.
+  Qed.
+
+  Lemma interp_cstr_shift {V v c} :
+    wf_zero_valuation V v ->
     declared_univ_cstr_levels V c ->
-    interp_nat_cstr v c -> interp_nat_cstr (shift_valuation v) c.
+    interp_nat_cstr v c <-> interp_nat_cstr (shift_valuation v) c.
   Proof.
     intros hfw hdecl.
     destruct c as [[l d] r]; cbn.
-    destruct d.
-    intros hi. *)
+    move: (interp_nes_shift (u := l) hfw) => /fwd. apply hdecl.
+    move=> [hl hle].
+    move: (interp_nes_shift (u := r) hfw) => /fwd. apply hdecl.
+    move=> [hr hre].
+    destruct d; rewrite hl hr; split; lia.
+  Qed.
 
+  Lemma declared_univ_cstr_levels_incl V c cls :
+    declared_univ_cstrs_levels V cls ->
+    UnivConstraintSet.In c cls ->
+    declared_univ_cstr_levels V c.
+  Proof.
+    now move=> hdecl /hdecl.
+  Qed.
+
+  Lemma interp_cstrs_shift V v c :
+    wf_zero_valuation V v ->
+    declared_univ_cstrs_levels V c ->
+    interp_cstrs v c <-> interp_cstrs (shift_valuation v) c.
+  Proof.
+    intros hfw hdecl.
+    split; move=> hv cl /[dup] hin /hv; rewrite (interp_cstr_shift hfw); tea => //.
+    all:now eapply declared_univ_cstr_levels_incl.
+  Qed.
+
+  Lemma uctx_subset :
+    LevelSet.Subset (univ_constraints_levels uctx.2) uctx.1.
+  Proof.
+    red in Huctx. destruct Huctx. red in H0. intros l hin. red in H0.
+    apply univ_constraints_levels_spec in hin as [cl [hin hincl]].
+    apply H0 in hin.
+    apply declared_univ_cstr_levels_spec in hin. now apply hin.
+  Qed.
 
   Lemma checkb_spec : check_spec checkb.
   Proof.
@@ -373,66 +472,18 @@ Section CheckLeq.
       intros [ii iu].
       specialize (hv (to_valuation (shift_valuation v))).
       rewrite (satisfies_interp_cstr_inv uctx.1) in hv.
-      apply wf_shift_valuation. exact ii. admit.
+      { apply wf_shift_valuation. apply wf_zero_valuation_init. exact ii. }
+      apply uctx_subset.
       forward hv.
-
-
-
-      red.
-      Print init_constraint_of_level.
-
-      red in hv. About to_val.
-      rewrite inte
-      rewrite interp_
-      rewrite -satisfies_interp_cstr.
-      apply clauses_sem_satisfies_equiv in sat.
-
-      have hi := interp_cstr_clauses_sem.
-      red in sat.
-      apply satisfies_clauses_sem_to_Z in sat.
-      rewrite interp_univ_cstr_to_opt_val.
-      rewrite interp_univ_cstrs_nat.
-      red in mc.
-      setoid_rewrite interp_cstrs_clauses_sem in mc.
-      specialize (mc (to_opt_val (valuation_to_Z v))).
-      eapply interp_cstr_clauses_sem.
-      forward mc. apply posv.
-      rewrite -interp_univ_cstr_to_opt_val. apply mc.
-      rewrite clauses_sem_to_opt_val.
-      apply satisfies_clauses_sem_to_Z.
-      destruct HG as [hlev hcstrs].
-      rewrite hcstrs. eapply satisfies_union. split => //.
-      eapply satisfies_init.
-    - rewrite check_completeness.
-      intros hv. red in hv.
-      destruct HG as [hlev hcstrs].
-      intros v vpos cs.
-      Print valuation.
-      red.
-      rewrite valid_Z_pos_nat_model => v.
-      rewrite hcstrs.
-      erewrite <-interp_univ_cstrs_nat.
-      Search wf_valuation.
-      rewrite interp_cstrs_union.
-      specialize (hv (valuation_of_opt_nat v)).
-      intros interp.
-      rewrite -interp_univ_cstrs_nat in interp.
-
-
-      setoid_rewrite <- clauses_sem_satisfies_equiv in hv.
-      red. intros v vcs.
-      rewrite interp_cstr_clauses_sem.
-      Search interp_univ_cstrs.
-      setoid_rewrite interp_cstrs_clauses_sem in hcls.
-      rewrite interp_cstr_clauses_sem. *)
-
-
-
-
-       Search LoopCheck.Impl.CorrectModel.clauses_sem.
-    specialize (HG c).
-
-
+      rewrite -interp_cstrs_shift. apply wf_zero_valuation_init. apply ii.
+      apply Huctx. exact iu.
+      rewrite satisfies0_interp_cstr_inv in hv.
+      apply wf_shift_valuation.
+      apply wf_zero_valuation_init => //.
+      now apply declared_univ_cstr_levels_spec.
+      erewrite interp_cstr_shift => //.
+      apply wf_zero_valuation_init => //. exact decl.
+  Qed.
 
   Lemma fold_right_xpred0 {A} (l : list A) : fold_right (fun _ => xpred0) false l = false.
   Proof using Type. induction l; simpl; auto. Qed.
@@ -453,6 +504,8 @@ Section CheckLeq.
     - cbn. apply check_correct.
   Qed.
 
+  Definition check_leqb_universe_spec := check_leqb_universe_spec_gen _ checkb_spec.
+
   Lemma check_eqb_universe_spec_gen check
      (check_correct : check_spec check)
      (l l' : Universe.t)
@@ -466,1223 +519,82 @@ Section CheckLeq.
     - cbn. apply check_correct.
   Qed.
 
-  Definition check_leqb_universe_spec := check_leqb_universe_spec_gen _ check_spec.
-
-  Definition check_eqb_universe := (check_eqb_universe_gen leqb_level_n).
-
-  Lemma check_eqb_universe_spec_gen leqb_level_n_gen
-      (leqb_correct : leqb_level_n_spec_gen leqb_level_n_gen)
-      (l1 l2 : Universe.t)
-      (Hu1  : gc_levels_declared l1)
-      (Hu2  : gc_levels_declared l2)
-    : check_eqb_universe_gen leqb_level_n_gen l1 l2 <-> gc_eq_universe uctx.2 l1 l2.
-  Proof using HC HG Huctx.
-    unfold check_eqb_universe_gen, gc_eq_universe.
-    destruct check_univs; [|split; trivial].
-    split; cbn.
-    - move/orP => [ | /andP [Hle Hge]].
-      + rewrite univ_expr_eqb_true_iff.
-        now intros <- v Hv.
-      + eapply leqb_universe_n_spec0_gen in Hle, Hge; eauto.
-        unfold_univ_rel0. specialize (Hle v Hv); specialize (Hge v Hv).
-        simpl in *. lia.
-    - intros H. toProp; right.
-      toProp; eapply leqb_universe_n_spec_gen; tas; intros v Hv; specialize (H v Hv).
-      rewrite H. cbn; lia.
-      rewrite H. cbn; lia.
-  Qed.
-
-  Definition check_eqb_universe_spec := check_eqb_universe_spec_gen _ leqb_level_n_spec.
+  Definition check_eqb_universe_spec := check_eqb_universe_spec_gen _ checkb_spec.
 
   Lemma fold_left_false {A} l : fold_left (B:=A) (fun _ : bool => xpred0) l false = false.
   Proof using Type.
     induction l; simpl; eauto.
   Qed.
 
-  Definition check_gc_constraint := (check_gc_constraint_gen leqb_level_n).
+  Definition check_constraints := (check_constraints_gen checkb).
+  Definition eqb_univ_instance := (eqb_univ_instance_gen checkb).
 
-  Definition check_gc_constraints := (check_gc_constraints_gen leqb_level_n).
+  Definition leqb_sort := (leqb_sort_gen checkb).
 
-  Definition check_constraints := (check_constraints_gen leqb_level_n).
+  Definition check_leqb_sort := (check_leqb_sort_gen checkb).
 
+  Definition check_eqb_sort := (check_eqb_sort_gen checkb).
 
-  Definition gc_levels_declared' (vset : VSet.t) gc :=
-     match gc with
-    | GoodConstraint.gc_le l _ l' => VSet.In (VariableLevel.to_noprop l) vset /\
-      VSet.In (VariableLevel.to_noprop l') vset
-    | GoodConstraint.gc_lt_set_level _ n | GoodConstraint.gc_le_level_set n _ =>
-	     VSet.In (Level.level  n) vset
-    | GoodConstraint.gc_le_set_var _ n | GoodConstraint.gc_le_var_set n _ => VSet.In (Level.lvar n) vset
-     end.
-
-  Definition gcs_levels_declared (vset : VSet.t) gcs :=
-    GoodUnivConstraintSet.For_all (gc_levels_declared' vset) gcs.
-
-
-  Lemma check_gc_constraint_spec_gen leqb_level_n_gen
-    (leqb_correct : leqb_level_n_spec_gen leqb_level_n_gen)
-    gc
-    (Hu1 : gc_levels_declared' uctx.1 gc)
-    : check_gc_constraint_gen leqb_level_n_gen gc
-      -> if check_univs then forall v, gc_satisfies v uctx.2 -> gc_satisfies0 v gc else True.
-  Proof using Huctx.
-    unfold check_gc_constraint_gen.
-    destruct check_univs; [cbn|trivial].
-    destruct gc as [l z l'|k l|k n|l k|n k].
-    - intros HH v Hv; eapply leqb_correct in HH; eauto.
-      specialize (HH v Hv). cbn in *. toProp.
-      pose proof (val_level_of_variable_level v l).
-      pose proof (val_level_of_variable_level v l').
-      destruct l, l'; cbn in *; lia.
-      all: now inversion Hu1.
-    - intros HH v Hv; eapply leqb_correct in HH; eauto.
-      specialize (HH v Hv). cbn -[Z.of_nat] in HH. unfold gc_satisfies0. toProp.
-      cbn in *. lia.
-      now inversion Huctx.
-    - intros HH v Hv; apply leqb_correct in HH.
-      specialize (HH v Hv). cbn in HH. unfold gc_satisfies0. toProp.
-      lia. now inversion Huctx. now inversion Hu1.
-    - intros HH v Hv; apply leqb_correct in HH.
-      specialize (HH v Hv). cbn in HH. unfold gc_satisfies0. toProp.
-      lia. now inversion Hu1. now inversion Huctx.
-    - intros HH v Hv; apply leqb_correct in HH.
-      specialize (HH v Hv). cbn in HH. unfold gc_satisfies0. toProp.
-      lia. now inversion Hu1. now inversion Huctx.
-  Qed.
-
-  Definition check_gc_constraint_spec := check_gc_constraint_spec_gen _ leqb_level_n_spec.
-
-  Lemma check_gc_constraints_spec_gen leqb_level_n_gen
-    (leqb_correct : leqb_level_n_spec_gen leqb_level_n_gen)
-    ctrs (Hu1 : gcs_levels_declared uctx.1 ctrs)
-    : check_gc_constraints_gen leqb_level_n_gen ctrs
-      -> if check_univs then forall v, gc_satisfies v uctx.2 -> gc_satisfies v ctrs else True.
-  Proof using Huctx.
-    rewrite /gcs_levels_declared in Hu1. pose proof check_gc_constraint_spec_gen as XX.
-    unfold check_gc_constraints_gen. destruct check_univs; [cbn|trivial].
-    intros HH v Hv.
-    apply GoodUnivConstraintSet.for_all_spec. now intros x y [].
-    apply GoodUnivConstraintSet.for_all_spec in HH. 2: now intros x y [].
-    intros gc Hgc. specialize (HH gc Hgc).
-    eapply XX; try eassumption. now apply Hu1.
-  Qed.
-
-  Definition check_gc_constraints_spec := check_gc_constraints_spec_gen _ leqb_level_n_spec.
-
-  Definition eqb_univ_instance := (eqb_univ_instance_gen leqb_level_n).
-
-  Definition leqb_sort := (leqb_sort_gen leqb_level_n).
-
-  Definition check_leqb_sort := (check_leqb_sort_gen leqb_level_n).
-
-  Definition check_eqb_sort := (check_eqb_sort_gen leqb_level_n).
-
-  Lemma check_eqb_sort_refl_gen leqb_level_n_gen
-    (leqb_correct : leqb_level_n_spec_gen leqb_level_n_gen) u :
-    check_eqb_sort_gen leqb_level_n_gen u u.
+  Lemma check_eqb_sort_refl_gen check
+    (leqb_correct : check_spec check) u :
+    check_eqb_sort_gen check u u.
   Proof using Type.
     unfold check_eqb_sort_gen; toProp; left.
     apply eqb_refl.
   Qed.
 
-  Definition check_eqb_sort_refl := check_eqb_sort_refl_gen _ leqb_level_n_spec.
+  Definition check_eqb_sort_refl := check_eqb_sort_refl_gen _ checkb_spec.
 
-  Definition gc_leq_sort φ :=
-    leq_sort_n_ (fun n u u' => if check_univs then gc_leq0_universe_n n φ u u' else True) 0.
+  (* Let levels_declared_sort (s : Sort.t) :=
+    Sort.on_sort gc_levels_declared True s. *)
 
-  Definition gc_eq_sort φ :=
-    eq_sort_ (fun u u' => if check_univs then gc_eq0_universe φ u u' else True).
+  Lemma levels_declared_uctx u : levels_declared u -> LevelSet.Subset (Universe.levels u) uctx.1.
+  Proof.
+    move=> hu l. hnf in hu.
+    rewrite Universe.levels_spec.
+    move=> -[k /hu hin]. apply hin.
+  Qed.
 
-  Let levels_declared_sort (s : Sort.t) :=
-    Sort.on_sort gc_levels_declared True s.
-
-  Lemma check_eqb_sort_spec_gen leqb_level_n_gen
-      (leqb_correct : leqb_level_n_spec_gen leqb_level_n_gen)
+  Lemma check_eqb_sort_spec_gen check
+      (leqb_correct : check_spec check)
       (u1 u2 : Sort.t)
       (Hu1 : levels_declared_sort u1)
       (Hu2 : levels_declared_sort u2)
-    : check_eqb_sort_gen leqb_level_n_gen u1 u2 <-> gc_eq_sort uctx.2 u1 u2.
+    : check_eqb_sort_gen check u1 u2 <-> eq_sort uctx.2 u1 u2.
   Proof.
-    unfold check_eqb_sort_gen, gc_eq_sort.
+    unfold check_eqb_sort_gen, eq_sort.
     destruct u1, u2; cbnr; split; intuition auto.
     - now destruct prop_sub_type.
-    - eapply check_eqb_universe_spec_gen; eauto; tas.
-      unfold check_eqb_sort_gen, check_eqb_universe_gen in *; cbn in *.
-      unfold check_leqb_universe_gen in *.
-      destruct check_univs; cbnr.
-      unfold eqb at 1, Sort.reflect_eq_sort, Sort.eqb in H. cbn in H.
-      move/orP : H => /= [-> //|] /andP[] /orP[-> //|] H1 /orP[e | H2].
-      1: apply NonEmptySetFacts.univ_expr_eqb_true_iff in e as ->.
-      1: toProp; left; now apply NonEmptySetFacts.univ_expr_eqb_true_iff.
-      toProp; right; now toProp.
+    - toProp. destruct H.
+      apply (@elimP _ _ (eqb_spec _ _)) in H. noconf H.
+      reflexivity.
+      toProp. destruct H as [hle hle'].
+      apply (check_leqb_universe_spec_gen _ leqb_correct) in hle'.
+      apply (check_leqb_universe_spec_gen _ leqb_correct) in hle.
+      unfold valid_cstr, valid0_cstr in hle, hle'.
+      apply antisymmetry; unfold Universes.leq_universe, Universes.leq0_universe;
+      destruct check_univs => //.
+      now move=> v /hle; intros s; depelim s.
+      now move=> v /hle'; intros s; depelim s.
+      all:split; now apply levels_declared_uctx.
     - toProp; right.
-      eapply check_eqb_universe_spec_gen in H; eauto; tas.
-      unfold check_eqb_universe_gen in *; cbn in *.
-      unfold check_leqb_universe_gen in *.
-      destruct check_univs; [cbn in * | trivial].
-      move/orP : H => [H | /andP [H1 H2]].
-      + apply NonEmptySetFacts.univ_expr_eqb_true_iff in H as ->.
-        toProp; toProp; left; now apply NonEmptySetFacts.univ_expr_eqb_true_iff.
-      + toProp; toProp; right; assumption.
-  Defined.
+      apply partial_order_equivalence in H as [H H'].
+      toProp; apply/(check_leqb_universe_spec_gen _ leqb_correct).
+      * split; now apply levels_declared_uctx.
+      * move: H; rewrite /Universes.leq_universe /Universes.leq0_universe.
+        unfold valid_cstr, valid0_cstr. destruct check_univs => //.
+        move=> hv v /hv. now constructor.
+      * split; now apply levels_declared_uctx.
+      * move: H'; rewrite /Universes.leq_universe /Universes.leq0_universe.
+        unfold valid_cstr, valid0_cstr. destruct check_univs => //.
+        move=> hv v /hv. now constructor.
+  Qed.
 
-  Definition check_eqb_sort_spec := check_eqb_sort_spec_gen _ leqb_level_n_spec.
+  Definition check_eqb_sort_spec := check_eqb_sort_spec_gen _ checkb_spec.
 
 End CheckLeq.
 
-(* This section: specif in term of raw uctx *)
-Section CheckLeq2.
-  Context {cf:checker_flags}.
-
-  Definition is_graph_of_uctx G uctx
-    := on_Some (fun uctx => Equal_graph (make_graph uctx) G) (gc_of_uctx uctx).
-
-  Context (G : universes_graph)
-          uctx (Huctx: global_uctx_invariants uctx) (HC : consistent uctx.2)
-          (HG : is_graph_of_uctx G uctx).
-
-  Definition uctx' : VSet.t × GoodUnivConstraintSet.t.
-    unfold is_graph_of_uctx, gc_of_uctx in HG.
-    destruct (gc_of_constraints uctx.2) as [ctrs|].
-    exact (uctx.1, ctrs).
-    contradiction HG.
-  Defined.
-
-  #[clearbody] Let Huctx' : global_gc_uctx_invariants uctx'.
-    unfold uctx'; cbn.
-    eapply gc_of_uctx_invariants; tea.
-    unfold is_graph_of_uctx, gc_of_uctx in *. cbn.
-    destruct (gc_of_constraints uctx.2) as [ctrs|].
-    reflexivity. contradiction HG.
-  Defined.
-
-  #[clearbody]
-  Let HC' : gc_consistent uctx'.2.
-    unfold uctx'; cbn. clear Huctx'.
-    apply gc_consistent_iff in HC.
-    unfold is_graph_of_uctx, gc_of_uctx in *.
-    destruct (gc_of_constraints uctx.2) as [ctrs|].
-    exact HC. contradiction HG.
-  Defined.
-
-  #[clearbody]
-  Let HG' : Equal_graph G (make_graph uctx').
-    unfold uctx' in *; cbn. clear Huctx'.
-    unfold is_graph_of_uctx, gc_of_uctx in *.
-    destruct (gc_of_constraints uctx.2) as [ctrs|].
-    symmetry; exact HG. contradiction HG.
-  Defined.
-
-  Let level_declared (l : Level.t) := LevelSet.In l uctx.1.
-
-  Let expr_declared (e : LevelExpr.t)
-    := on_Some_or_None (fun l : Level.t => level_declared l)
-                       (LevelExpr.get_noprop e).
-
-  Let levels_declared (u : Universe.t) :=
-    LevelExprSet.For_all expr_declared u.
-
-  Lemma level_gc_declared_declared l
-    : level_declared l -> gc_level_declared uctx' l.
-  Proof using HG.
-    clear. unfold uctx'.
-    unfold is_graph_of_uctx, gc_of_uctx in HG.
-    destruct (gc_of_constraints uctx.2); [|contradiction HG].
-    cbn; clear HG. unfold level_declared, gc_level_declared; cbn.
-    destruct l; cbn; trivial; intro.
-  Qed.
-
-  Lemma expr_gc_declared_declared e
-    : expr_declared e -> gc_expr_declared uctx' e.
-  Proof using HG level_declared.
-    destruct e as [l b]; cbn; trivial.
-    intro; now apply (level_gc_declared_declared l) in H.
-  Qed.
-
-  Lemma levels_gc_declared_declared (u : Universe.t)
-    : levels_declared u -> gc_levels_declared uctx' u.
-  Proof using HG expr_declared.
-    unfold levels_declared, gc_levels_declared.
-    intros HH e He; specialize (HH e He).
-    now apply expr_gc_declared_declared.
-  Qed.
-
-  Lemma leqb_univ_expr_n_spec_gen' leqb_level_n_gen
-        (leqb_correct : leqb_level_n_spec_gen uctx' leqb_level_n_gen)
-        lt e1 u
-        (He1 : expr_declared e1)
-        (Hu : levels_declared u)
-    : leqb_expr_univ_n_gen leqb_level_n_gen ⎩ lt ⎭ e1 u
-      <-> leq0_universe_n ⎩ lt ⎭ uctx.2 (Universe.make e1) u.
-  Proof using HG' Huctx'.
-    etransitivity.
-    eapply (leqb_expr_univ_n_spec_gen G uctx' Huctx' HC' HG'); eauto; tas.
-    - apply expr_gc_declared_declared; tas.
-    - apply levels_gc_declared_declared; tas.
-    - symmetry. etransitivity. apply gc_leq0_universe_n_iff.
-      unfold uctx'; cbn; clear -HG.
-      unfold is_graph_of_uctx, gc_of_uctx in *.
-      destruct (gc_of_constraints uctx.2) as [ctrs|].
-      reflexivity. contradiction HG.
-  Qed.
-
-  Definition leqb_univ_expr_n_spec' :=
-      leqb_univ_expr_n_spec_gen' _ (leqb_level_n_spec _ _ Huctx' HC' HG').
-
-  Lemma check_leqb_universe_spec_gen' leqb_level_n_gen
-      (leqb_correct : leqb_level_n_spec_gen uctx' leqb_level_n_gen)
-      u1 u2
-    : levels_declared u1 ->
-      levels_declared u2 ->
-      check_leqb_universe_gen leqb_level_n_gen u1 u2 -> leq_universe uctx.2 u1 u2.
-  Proof using HG' Huctx'.
-    unfold check_leqb_universe_gen; intros Hu1 Hu2 H.
-    unfold_univ_rel.
-    cbn in H; toProp H; destruct H as [e | ].
-    { apply NonEmptySetFacts.univ_expr_eqb_true_iff in e. destruct e; lia. }
-    eapply leqb_universe_n_spec0_gen in H; eauto.
-    eapply gc_leq0_universe_iff; tea.
-    unfold uctx' in *.
-    unfold is_graph_of_uctx, gc_of_uctx in HG.
-    destruct (gc_of_constraints uctx.2). cbn in *. exact H.
-    exact I.
-    Unshelve. all: try eapply levels_gc_declared_declared; eauto.
-  Qed.
-
-  Definition check_leqb_universe_spec' :=
-    check_leqb_universe_spec_gen' _ (leqb_level_n_spec _ _ Huctx' HC' HG').
-
-  Lemma check_leqb_universe_complete_gen leqb_level_n_gen
-    (leqb_correct : leqb_level_n_spec_gen uctx' leqb_level_n_gen) u1 u2 :
-    levels_declared u1 ->
-    levels_declared u2 ->
-    leq_universe uctx.2 u1 u2 ->
-    check_leqb_universe_gen leqb_level_n_gen u1 u2.
-  Proof using HG' Huctx'.
-    intros decl1 decl2.
-    apply levels_gc_declared_declared in decl1.
-    apply levels_gc_declared_declared in decl2.
-    rewrite gc_leq_universe_iff.
-    unfold is_graph_of_uctx, gc_of_uctx in HG.
-    unfold uctx' in *.
-    destruct gc_of_constraints; [cbn in *|contradiction HG].
-    intros eq.
-    apply <- check_leqb_universe_spec_gen; eauto.
-    exact eq.
-  Qed.
-
-  Definition check_leqb_universe_complete :=
-    check_leqb_universe_complete_gen _ (leqb_level_n_spec _ _ Huctx' HC' HG').
-
-  Lemma check_eqb_universe_spec_gen' leqb_level_n_gen
-      (leqb_correct : leqb_level_n_spec_gen uctx' leqb_level_n_gen)
-      u1 u2
-    : levels_declared u1 ->
-      levels_declared u2 ->
-      check_eqb_universe_gen leqb_level_n_gen u1 u2 -> eq_universe uctx.2 u1 u2.
-  Proof using HG' Huctx'.
-    unfold check_eqb_universe_gen; intros Hu1 Hu2 H.
-    unfold_univ_rel.
-    cbn in H; toProp H; destruct H as [e | ].
-    { apply NonEmptySetFacts.univ_expr_eqb_true_iff in e. destruct e; lia. }
-    apply andb_prop in H. destruct H as [H1 H2].
-    unshelve eapply leqb_universe_n_spec0_gen in H1; eauto.
-    unshelve eapply leqb_universe_n_spec0_gen in H2; eauto.
-    unfold uctx' in *.
-    unfold is_graph_of_uctx, gc_of_uctx in HG.
-    apply <- eq0_leq0_universe; tea.
-    split; eapply gc_leq0_universe_iff;
-      (destruct (gc_of_constraints uctx.2); [cbn in *|contradiction HG]); tas.
-    all: now eapply levels_gc_declared_declared.
-  Qed.
-
-  Definition check_eqb_universe_spec' :=
-    check_eqb_universe_spec_gen' _ (leqb_level_n_spec _ _ Huctx' HC' HG').
-
-  Lemma check_eqb_universe_complete_gen leqb_level_n_gen
-    (leqb_correct : leqb_level_n_spec_gen uctx' leqb_level_n_gen) u1 u2 :
-    levels_declared u1 ->
-    levels_declared u2 ->
-    eq_universe uctx.2 u1 u2 ->
-    check_eqb_universe_gen leqb_level_n_gen u1 u2.
-  Proof using HG' Huctx'.
-    intros decl1 decl2.
-    apply levels_gc_declared_declared in decl1.
-    apply levels_gc_declared_declared in decl2.
-    rewrite gc_eq_universe_iff.
-    unfold is_graph_of_uctx, gc_of_uctx in HG.
-    unfold uctx' in *.
-    destruct gc_of_constraints; [cbn in *|contradiction HG].
-    intros eq.
-    apply <- check_eqb_universe_spec_gen; eauto.
-    exact eq.
-  Qed.
-
-  Definition check_eqb_universe_complete :=
-    check_eqb_universe_complete_gen _ (leqb_level_n_spec _ _ Huctx' HC' HG').
-
-  Definition leq0_level_n z l l' :=
-    leq0_universe_n z uctx.2 (Universe.make' l) (Universe.make' l').
-
-  Definition valid_gc_constraint (gc : GoodConstraint.t) :=
-    match gc with
-    | GoodConstraint.gc_le l z l' => leq0_level_n z l l'
-    | GoodConstraint.gc_lt_set_level k l => leq0_level_n (Z.of_nat (S k)) lzero (Level.level  l)
-    | GoodConstraint.gc_le_set_var k n => leq0_level_n (Z.of_nat k) lzero (Level.lvar n)
-    | GoodConstraint.gc_le_level_set l k => leq0_level_n (- Z.of_nat k)%Z (Level.level  l) lzero
-    | GoodConstraint.gc_le_var_set n k => leq0_level_n (- Z.of_nat k)%Z (Level.lvar n) lzero
-    end.
-
-  Definition valid_gc_constraints (gcs : GoodUnivConstraintSet.t) :=
-    GoodUnivConstraintSet.For_all valid_gc_constraint gcs.
-
-  Lemma leq0_level_n_complete_gen leqb_level_n_gen
-    (leqb_correct : leqb_level_n_spec_gen uctx' leqb_level_n_gen) z l l' :
-    level_declared l ->
-    level_declared l' ->
-    leq0_level_n z l l' ->
-    leqb_level_n_gen z l l'.
-  Proof using HG' Huctx'.
-    intros decll decll'.
-    unfold leq0_level_n.
-    intros le; eapply gc_leq0_universe_n_iff in le.
-    unfold is_graph_of_uctx, gc_of_uctx in HG.
-    unfold uctx' in *.
-    destruct gc_of_constraints; [cbn in *|contradiction HG].
-    now eapply leqb_correct.
-  Qed.
-
-  Definition leq0_level_n_complete :=
-    leq0_level_n_complete_gen _ (leqb_level_n_spec _ _ Huctx' HC' HG').
-
-  Lemma check_gc_constraint_complete_gen leqb_level_n_gen
-    (leqb_correct : leqb_level_n_spec_gen uctx' leqb_level_n_gen) cstr :
-    gc_levels_declared' uctx.1 cstr ->
-    valid_gc_constraint cstr ->
-    check_gc_constraint_gen leqb_level_n_gen cstr.
-  Proof using HG' Huctx'.
-    rewrite /check_gc_constraint_gen.
-    destruct check_univs eqn:cu => //=.
-    destruct cstr; cbn; intros hin;
-    eapply leq0_level_n_complete_gen; intuition auto.
-    all:apply Huctx.
-  Qed.
-
-  Definition check_gc_constraint_complete :=
-    check_gc_constraint_complete_gen _ (leqb_level_n_spec _ _ Huctx' HC' HG').
-
-  Lemma check_gc_constraints_complete_gen leqb_level_n_gen
-    (leqb_correct : leqb_level_n_spec_gen uctx' leqb_level_n_gen) cstrs :
-    gcs_levels_declared uctx.1 cstrs ->
-    valid_gc_constraints cstrs ->
-    check_gc_constraints_gen leqb_level_n_gen cstrs.
-  Proof using HG' Huctx'.
-    rewrite /gcs_levels_declared /valid_gc_constraints /check_gc_constraints.
-    intros hdecl hval.
-    eapply GoodConstraintSetFact.for_all_iff. typeclasses eauto.
-    intros cstr hcstr. specialize (hdecl cstr hcstr).
-    specialize (hval cstr hcstr). eapply check_gc_constraint_complete_gen => //.
-  Qed.
-
-  Definition check_gc_constraints_complete :=
-    check_gc_constraints_complete_gen _ (leqb_level_n_spec _ _ Huctx' HC' HG').
-
-  Definition valid_gc_constraints_ext gc :=
-    forall v, satisfies v uctx.2 -> gc_satisfies v gc.
-
-  Lemma valid_gc_constraints_aux gc :
-    valid_gc_constraints_ext gc ->
-    valid_gc_constraints gc.
-  Proof using Type.
-    intros Hv v inv.
-    unfold gc_satisfies in Hv.
-    destruct v; cbn in *; red;
-    intros v Hv'; specialize (Hv _ Hv');
-    eapply GoodConstraintSetFact.for_all_iff in Hv; try typeclasses eauto;
-    specialize (Hv _ inv); cbn in Hv; cbn;
-    rewrite ?val_level_of_variable_level //.
-
-    now eapply Z.leb_le in Hv.
-    eapply Nat.leb_le in Hv. lia.
-    apply Nat.leb_le in Hv. lia.
-    apply Nat.leb_le in Hv. lia.
-    apply Nat.leb_le in Hv. lia.
-  Qed.
-
-  Lemma valid_valid_gc cstrs gc :
-    check_univs ->
-    valid_constraints uctx.2 cstrs ->
-    gc_of_constraints cstrs = Some gc ->
-    valid_gc_constraints gc.
-  Proof using Type.
-    intros cu Hgc vgc. apply valid_gc_constraints_aux.
-    intros v Hv.
-    pose proof (gc_of_constraints_spec v cstrs).
-    rewrite vgc /= in H. apply H.
-    rewrite /valid_constraints cu in Hgc. apply Hgc. apply Hv.
-  Qed.
-
-  Lemma gc_of_constraints_declared cstrs levels gc :
-    global_uctx_invariants (levels, cstrs) ->
-    gc_of_constraints cstrs = Some gc ->
-    gcs_levels_declared levels gc.
-  Proof using Type.
-    intros Hlev hc.
-    pose proof (gc_of_uctx_invariants (levels, cstrs) (levels, gc)).
-    cbn in H. rewrite hc in H. specialize (H eq_refl). now apply H.
-  Qed.
-
-  Lemma check_constraints_spec_gen  leqb_level_n_gen
-    (leqb_correct : leqb_level_n_spec_gen uctx' leqb_level_n_gen) ctrs
-    : global_uctx_invariants (uctx.1, ctrs) ->
-      check_constraints_gen leqb_level_n_gen ctrs -> valid_constraints uctx.2 ctrs.
-  Proof using HG' Huctx'.
-    unfold check_constraints_gen, valid_constraints.
-    case_eq (gc_of_constraints ctrs); [|try discriminate].
-    intros ctrs' Hctrs' Hdeclared HH.
-    epose proof check_gc_constraints_spec_gen.
-    destruct check_univs => //=.
-    intros v Hv.
-    apply gc_of_constraints_spec.
-    apply gc_of_constraints_spec in Hv.
-    rewrite Hctrs'; cbn. eapply H; eauto;
-    clear -HG Hv Hdeclared Hctrs';
-    unfold is_graph_of_uctx, gc_of_uctx in HG;
-    unfold uctx' in *; destruct (gc_of_constraints uctx.2) => //; cbn in *.
-    eapply gc_of_constraints_declared; eauto.
-  Qed.
-
-  Definition check_constraints_spec :=
-    check_constraints_spec_gen _ (leqb_level_n_spec _ _ Huctx' HC' HG').
-
-  (* Completeness holds only for well-formed constraints sets *)
-  Lemma check_constraints_complete_gen leqb_level_n_gen
-    (leqb_correct : leqb_level_n_spec_gen uctx' leqb_level_n_gen) ctrs :
-    check_univs ->
-    global_uctx_invariants (uctx.1, ctrs) ->
-    valid_constraints uctx.2 ctrs ->
-    check_constraints_gen leqb_level_n_gen ctrs.
-  Proof using HG' Huctx'.
-    intros cu gu vc.
-    unfold check_constraints_gen.
-    case_eq (gc_of_constraints ctrs); [|try discriminate].
-    2:{ destruct HC as [v Hv].
-        pose proof (gc_of_constraints_spec v ctrs).
-        intros.
-        rewrite /valid_constraints cu in vc.
-        specialize (vc v Hv).
-        rewrite H0 in H. intuition. }
-    intros cstr gc.
-    eapply check_gc_constraints_complete_gen; eauto.
-    { eapply gc_of_constraints_declared. 2:tea. cbn. red in gu.  unfold is_graph_of_uctx, gc_of_uctx in HG.
-      unfold uctx' in *.
-      destruct (gc_of_constraints uctx.2) => //; cbn in uctx', HG. }
-    eapply valid_valid_gc; tea.
-  Qed.
-
-  Definition check_constraints_complete :=
-    check_constraints_complete_gen _ (leqb_level_n_spec _ _ Huctx' HC' HG').
-
-  Let levels_declared_sort (s : Sort.t)
-    := Sort.on_sort levels_declared True s.
-
-  Lemma levels_univ_gc_declared_declared (s : Sort.t)
-    : levels_declared_sort s -> gc_levels_declared_sort uctx' s.
-  Proof using HG levels_declared.
-    destruct s; cbnr.
-    apply levels_gc_declared_declared.
-  Qed.
-
-  Lemma check_leqb_sort_spec_gen' leqb_level_n_gen
-    (leqb_correct : leqb_level_n_spec_gen uctx' leqb_level_n_gen) s1 s2
-    : levels_declared_sort s1 ->
-      levels_declared_sort s2 ->
-      check_leqb_sort_gen leqb_level_n_gen s1 s2 -> leq_sort uctx.2 s1 s2.
-  Proof using HG' Huctx'.
-    intros Hu1 Hu2. move => /orP [H | H].
-    - apply eqb_true_iff in H as ->.
-      reflexivity.
-    - destruct s1, s2; cbn in *; trivial; try discriminate H.
-      now eapply check_leqb_universe_spec_gen'.
-  Qed.
-
-  Definition check_leqb_sort_spec' :=
-    check_leqb_sort_spec_gen' _ (leqb_level_n_spec _ _ Huctx' HC' HG').
-
-  Lemma check_leqb_sort_complete_gen leqb_level_n_gen
-    (leqb_correct : leqb_level_n_spec_gen uctx' leqb_level_n_gen) s1 s2 :
-    levels_declared_sort s1 ->
-    levels_declared_sort s2 ->
-    leq_sort uctx.2 s1 s2 ->
-    check_leqb_sort_gen leqb_level_n_gen s1 s2.
-  Proof using HG' Huctx'.
-    move : s1 s2 => [| | u1] [| | u2] //. cbn.
-    intros decl1 decl2 Hle.
-    unfold check_leqb_sort_gen.
-    toProp; right.
-    apply check_leqb_universe_complete_gen => //.
-  Qed.
-
-  Definition check_leqb_sort_complete :=
-    check_leqb_sort_complete_gen _ (leqb_level_n_spec _ _ Huctx' HC' HG').
-
-  Lemma check_eqb_sort_spec_gen' leqb_level_n_gen
-    (leqb_correct : leqb_level_n_spec_gen uctx' leqb_level_n_gen) s1 s2
-    : levels_declared_sort s1 ->
-      levels_declared_sort s2 ->
-      check_eqb_sort_gen leqb_level_n_gen s1 s2 -> eq_sort uctx.2 s1 s2.
-  Proof using HG' Huctx'.
-    move : s1 s2 => [| | u1] [| | u2] //; intros Hu1 Hu2.
-    { move/andP => [H HH] //. }
-    move/orP => [H | H].
-    - apply eqb_true_iff in H as ->.
-      reflexivity.
-    - eapply check_eqb_universe_spec_gen'; eauto.
-      cbn in H. unfold check_eqb_universe_gen in *.
-      move/andP: H => [/orP [/orP [-> | ->] | ->] /orP [/orP [He | HH] | ->]] //.
-      all: try now rewrite orb_true_r.
-      now rewrite He.
-      apply NonEmptySetFacts.univ_expr_eqb_true_iff in HH as ->.
-      toProp; left; toProp; right; now apply NonEmptySetFacts.univ_expr_eqb_true_iff.
-  Qed.
-
-  Definition check_eqb_sort_spec' :=
-    check_eqb_sort_spec_gen' _ (leqb_level_n_spec _ _ Huctx' HC' HG').
-
-  Lemma check_eqb_sort_complete_gen leqb_level_n_gen
-    (leqb_correct : leqb_level_n_spec_gen uctx' leqb_level_n_gen) u1 u2 :
-    levels_declared_sort u1 ->
-    levels_declared_sort u2 ->
-    eq_sort uctx.2 u1 u2 ->
-    check_eqb_sort_gen leqb_level_n_gen u1 u2.
-  Proof using HG' Huctx'.
-    move : u1 u2 => [| | u1] [| | u2] //. cbn.
-    intros decl1 decl2 Hle.
-    eapply check_eqb_universe_complete_gen in Hle => //; eauto.
-    unfold check_eqb_sort_gen, leqb_sort_gen, check_leqb_universe_gen; cbn.
-    unfold check_eqb_universe_gen in Hle.
-    move/orP: Hle => [/orP [-> | e] | /andP [H1 H2]] //=.
-    now rewrite orb_true_r.
-    apply eqb_eq in e as ->; rewrite eqb_refl //.
-    toProp; right; toProp; toProp; right; assumption.
-  Qed.
-
-  Definition check_eqb_sort_complete :=
-    check_eqb_sort_complete_gen _ (leqb_level_n_spec _ _ Huctx' HC' HG').
-
-End CheckLeq2.
-
-Section AddLevelsCstrs.
-
-  Definition add_uctx (uctx : VSet.t × GoodUnivConstraintSet.t)
-             (G : universes_graph) : universes_graph
-    := let levels := VSet.union uctx.1 G.1.1 in
-       let edges := add_level_edges uctx.1 G.1.2 in
-       let edges := add_cstrs uctx.2 edges in
-       (levels, edges, G.2).
-
-  Definition uctx_of_udecl u : ContextSet.t :=
-    (levels_of_udecl u, constraints_of_udecl u).
-
-  Lemma gcs_elements_union s s' : GoodUnivConstraintSet.Empty s' ->
-    GoodUnivConstraintSet.Equal (GoodUnivConstraintSet.union s s') s.
-  Proof. gcsets. Qed.
-
-  Lemma add_level_edges_spec e x g :
-    EdgeSet.In e (add_level_edges x g) <->
-    (exists c, option_edge_of_level c = Some e /\ VSet.In c x) \/ EdgeSet.In e g.
-  Proof.
-    rewrite /add_level_edges VSet.fold_spec.
-    setoid_rewrite (VSetFact.elements_iff x). setoid_rewrite InA_In_eq.
-    induction (VSet.elements x) in g |- *; simpl.
-    intuition auto. now destruct H0 as [c [_ F]].
-    rewrite {}IHl.
-    split.
-    * intros [[c [eq inl]]|?]; firstorder auto.
-      destruct a as [|s|n]; simpl in *; auto.
-      rewrite -> EdgeSet.add_spec in H. intuition auto.
-      subst e. left; exists (Level.level  s); intuition auto.
-      rewrite -> EdgeSet.add_spec in H. intuition auto.
-      subst e. left; eexists; intuition eauto. reflexivity.
-    * intros [[[|s|n] [[= <-] [->|inl]]]|?]; simpl; auto;
-      rewrite -> ?EdgeSet.add_spec; simpl; intuition auto.
-      left. exists (Level.level  s); auto.
-      left. exists (Level.lvar n); auto.
-      destruct a; simpl; rewrite -> ?EdgeSet.add_spec; simpl; intuition auto.
-  Qed.
-
-  Lemma add_cstrs_union g ctrs1 ctrs2 :
-    EdgeSet.Equal (add_cstrs (GoodUnivConstraintSet.union ctrs1 ctrs2) g) (add_cstrs ctrs1 (add_cstrs ctrs2 g)).
-  Proof.
-    intros e.
-    rewrite !add_cstrs_spec.
-    setoid_rewrite GoodUnivConstraintSet.union_spec.
-    firstorder eauto.
-  Qed.
-
-  Lemma add_level_edges_union g l1 l2 :
-    EdgeSet.Equal (add_level_edges (VSet.union l1 l2) g)
-    (add_level_edges l1 (add_level_edges l2 g)).
-  Proof.
-    intros e.
-    rewrite !add_level_edges_spec.
-    setoid_rewrite VSet.union_spec.
-    firstorder eauto.
-  Qed.
-
-  Lemma add_level_edges_add_cstrs_comm l c g :
-    EdgeSet.Equal (add_level_edges l (add_cstrs c g))
-      (add_cstrs c (add_level_edges l g)).
-  Proof.
-    intros e.
-    rewrite !add_level_edges_spec !add_cstrs_spec add_level_edges_spec.
-    firstorder auto.
-  Qed.
-
-  Lemma forallb_spec {A : Type} (p : A -> bool) (l : list A) :
-    match forallb p l with
-    | true => forall x : A, In x l -> p x
-    | false => exists x : A, In x l × p x = false
-    end.
-  Proof.
-    induction l; cbn.
-    - now intros.
-    - destruct (forallb p l) eqn:heq.
-      rewrite andb_true_r.
-      destruct (p a) eqn:he.
-      intros x []. subst; auto. now apply IHl.
-      exists a; auto.
-      rewrite andb_false_r. destruct IHl as [x [inx hx]].
-      exists x. intuition auto.
-  Qed.
-
-  Lemma forallb_in {A : Type} (p : A -> bool) (l l' : list A) :
-    (forall x : A, In x l <-> In x l') ->
-    forallb p l = forallb p l'.
-  Proof.
-    intros heq.
-    generalize (forallb_spec p l).
-    generalize (forallb_spec p l').
-    do 2 destruct forallb; intuition auto.
-    destruct H0 as [x [hin hp]].
-    - specialize (H x (proj1 (heq x) hin)). red in H; congruence.
-    - destruct H as [x [hin hp]].
-      specialize (H0 x (proj2 (heq _) hin)). congruence.
-  Qed.
-
-  Lemma levelset_for_all_eq f f' l l' :
-    (forall x, f x = f' x) -> LevelSet.Equal l l' ->
-    LevelSet.for_all f l = LevelSet.for_all f' l'.
-  Proof.
-    intros Hf heq.
-    rewrite !VSetFact.for_all_b.
-    setoid_replace f with f'; auto.
-    eapply forallb_in.
-    intros x.
-    red in heq.
-    specialize (heq x).
-    rewrite -!InA_In_eq.
-    now rewrite -!LevelSetFact.elements_iff.
-  Qed.
-
-  Lemma Nbar_max_spec n m v :
-    Nbar.max n m = v ->
-    (Nbar.le n m /\ v = m) \/ (Nbar.le m n /\ v = n).
-  Proof.
-    destruct n, m; cbn; firstorder.
-    destruct (Z.max_spec_le z z0); firstorder; try lia.
-    left. split; auto. congruence.
-    right. split; auto. congruence.
-  Qed.
-
-  Lemma Nbar_max_spec' n m :
-    Nbar.le n m -> Nbar.max m n = m.
-  Proof.
-    destruct n, m; cbn; firstorder. f_equal. lia.
-  Qed.
-
-  Lemma Nbar_max_spec'' n m :
-    Nbar.le n m -> Nbar.max n m = m.
-  Proof.
-    destruct n, m; cbn; firstorder. f_equal. lia.
-  Qed.
-
-  Lemma Nbar_max_le n m k : Nbar.le (Nbar.max n m) k ->
-    Nbar.le n k /\ Nbar.le m k.
-  Proof.
-    intros hl.
-    generalize (Nbar_max_spec n m _ eq_refl). intuition subst; try rewrite H1 in hl; auto.
-    - now transitivity m.
-    - now transitivity n.
-  Qed.
-
-  Lemma fold_left_max_spec (l : list Nbar.t) acc n :
-    fold_left Nbar.max l acc = n ->
-    (n = acc /\ (forall x, In x l -> Nbar.le x n)) \/
-    (In n l /\ Nbar.le acc n /\ (forall x, In x l -> Nbar.le x n)).
-  Proof.
-    induction l in acc, n |- *.
-    - cbn. intros ->; firstorder.
-    - cbn. intros H. specialize (IHl _ _ H).
-      destruct IHl. firstorder auto.
-      symmetry in H0. apply Nbar_max_spec in H0.
-      firstorder auto. right. firstorder auto. subst; auto. now rewrite H2. subst x n.
-      rewrite H2. reflexivity.
-      left. firstorder auto. subst x n. now rewrite H2.
-      destruct H0.
-      right. firstorder auto.
-      now apply Nbar_max_le in H1.
-      now apply Nbar_max_le in H1.
-  Qed.
-
-
-  Lemma fold_left_max_spec' (l : list Nbar.t) acc n :
-    (n = acc /\ (forall x, In x l -> Nbar.le x n)) \/
-    (In n l /\ Nbar.le acc n /\ (forall x, In x l -> Nbar.le x n)) ->
-    fold_left Nbar.max l acc = n.
-  Proof.
-    induction l in acc, n |- *.
-    - cbn. intuition.
-    - cbn. intros H.
-      apply IHl. intuition auto.
-      subst acc.
-      pose proof (H1 a). left. split. symmetry. eapply Nbar_max_spec'; auto.
-      intuition auto.
-      left. split; intuition auto. subst a.
-      symmetry. now apply Nbar_max_spec''.
-      right. intuition auto. specialize (H2 a).
-      apply Nbar.max_lub; auto.
-  Qed.
-
-  Lemma fold_left_comm_ext (l l' : list Nbar.t) :
-    (forall x, In x l <-> In x l') ->
-    fold_left Nbar.max l ≐1 fold_left Nbar.max l'.
-  Proof.
-    intros eql acc.
-    generalize (fold_left_max_spec l acc _ eq_refl).
-    generalize (fold_left_max_spec l' acc _ eq_refl).
-    intuition auto.
-    - now rewrite H H0.
-    - rewrite H. apply fold_left_max_spec'. left; intuition auto.
-      specialize (H2 x (proj1 (eql _) H3)). congruence.
-    - rewrite H0. symmetry.
-      apply fold_left_max_spec'. left; intuition auto.
-      specialize (H4 x (proj2 (eql _) H2)). congruence.
-    - apply fold_left_max_spec'. right.
-      intuition auto. now apply eql. now apply H3, eql.
-  Qed.
-
-  Lemma fold_left_comm_ext2 f f' (l l' : list (Z × Level.t)) : f ≐1 f' ->
-    (forall x, In x l <-> In x l') ->
-    fold_left Nbar.max (map f l) ≐1 fold_left Nbar.max (map f' l').
-  Proof.
-    intros eqf eqg.
-    apply fold_left_comm_ext.
-    intros.
-    rewrite !in_map_iff. firstorder eauto.
-    specialize (eqg x0). exists x0; intuition auto. now rewrite -eqf.
-    exists x0. specialize (eqg x0). rewrite eqf; intuition auto.
-  Qed.
-
-  Lemma Equal_graph_edges {e e'} : Equal_graph e e' ->
-    forall x, In x (EdgeSet.elements e.1.2) <-> In x (EdgeSet.elements e'.1.2).
-  Proof.
-    intros [vs [es ?]]. intros x. red in vs.
-    now rewrite -!InA_In_eq -!EdgeSetFact.elements_iff.
-  Qed.
-
-  Lemma succs_proper x e e' v: Equal_graph e e' ->
-    In x (succs e v) <-> In x (succs e' v).
-  Proof.
-    intros eq. unfold succs.
-    rewrite !in_map_iff.
-    setoid_rewrite filter_In.
-    now setoid_rewrite (Equal_graph_edges eq).
-  Qed.
-
-  Lemma fold_left_comm_ext3 f f' e e' x : f ≐1 f' ->
-    Equal_graph e e' ->
-    fold_left Nbar.max (map f (succs e x)) ≐1
-    fold_left Nbar.max (map f' (succs e' x)).
-  Proof.
-    intros eqf eqg.
-    apply fold_left_comm_ext2; auto.
-    intros. now apply succs_proper.
-  Qed.
-
-  #[global] Instance lsp_proper : Morphisms.Proper ((=_g) ==> Logic.eq ==> Logic.eq ==> Logic.eq)%signature lsp.
-  Proof.
-    intros e e' He x ? <- y ? <-.
-    unfold lsp, lsp0.
-    pose proof (proj1 He).
-    change (wGraph.V e) with e.1.1.
-    change (wGraph.V e') with e'.1.1.
-    replace (LevelSet.cardinal e'.1.1) with (LevelSet.cardinal e.1.1).
-    2:{ now rewrite H. }
-    revert H.
-    generalize e.1.1, e'.1.1. intros t0 t1.
-    induction (LevelSet.cardinal t0) in t0, t1, e, e', He, x, y |- *. cbn; auto.
-    cbn. intros eqt.
-    replace (LevelSet.mem x t0) with (LevelSet.mem x t1).
-    2:{ now rewrite eqt. }
-    destruct LevelSet.mem; auto.
-    apply fold_left_comm_ext3; auto.
-    intros [n0 y0]. f_equal.
-    apply (IHn e e' He).
-    intros elt. rewrite !LevelSet.remove_spec.
-    intuition auto. now apply eqt. now apply eqt.
-  Qed.
-
-  #[global] Instance is_acyclic_proper : Morphisms.Proper ((=_g) ==> Logic.eq)%signature is_acyclic.
-  Proof.
-    intros e e' eq.
-    unfold is_acyclic.
-    eapply levelset_for_all_eq; tea. cbn.
-    intros x. now setoid_rewrite eq.
-    apply eq.
-  Qed.
-
-  Lemma add_uctx_make_graph levels1 levels2 ctrs1 ctrs2 :
-    Equal_graph (add_uctx (levels1, ctrs1) (make_graph (levels2, ctrs2)))
-      (make_graph (VSet.union levels1 levels2,
-                    GoodUnivConstraintSet.union ctrs1 ctrs2)).
-  Proof.
-    rewrite /make_graph /= /add_uctx /=.
-    unfold Equal_graph. split => //. split => //.
-    now rewrite add_cstrs_union /= add_level_edges_add_cstrs_comm add_level_edges_union.
-  Qed.
-
-  Lemma add_uctx_subgraph uctx G : subgraph G (add_uctx uctx G).
-  Proof.
-    constructor.
-    - apply: VSetProp.union_subset_2.
-    - move=> x hx.
-      apply/add_cstrs_spec; right.
-      apply/add_level_edges_spec; by right.
-    - reflexivity.
-  Qed.
-
-  Lemma acyclic_no_loop_add_uctx G uctx :
-    wGraph.acyclic_no_loop (add_uctx uctx G) -> wGraph.acyclic_no_loop G.
-  Proof.
-    apply: wGraph.subgraph_acyclic ; apply: add_uctx_subgraph.
-  Qed.
-
-  Definition gc_result_eq (x y : option GoodUnivConstraintSet.t) :=
-    match x, y with
-    | Some x, Some y => GoodUnivConstraintSet.eq x y
-    | None, None => True
-    | _, _ => False
-    end.
-
-  Lemma add_gc_of_constraint_spec {cf:checker_flags} gc t :
-    match add_gc_of_constraint gc (Some t) with
-    | Some t' =>
-      exists gcs, gc_of_constraint gc = Some gcs /\
-      GCS.Equal t' (GCS.union t gcs)
-    | None => gc_of_constraint gc = None
-    end.
-  Proof.
-    unfold add_gc_of_constraint.
-    simpl.
-    destruct gc_of_constraint; simpl; auto.
-    eexists; split; eauto. reflexivity.
-  Qed.
-
-  Lemma fold_left_add_gc_None {cf:checker_flags} l : fold_left (fun a e => add_gc_of_constraint e a) l None = None.
-  Proof.
-    induction l; simpl; auto.
-  Qed.
-
-  Lemma fold_left_add_gc_Some_subset {cf:checker_flags} l t t':
-    fold_left (fun a e => add_gc_of_constraint e a) l (Some t) = Some t' ->
-    GCS.Subset t t'.
-  Proof.
-    induction l in t |- *; simpl; auto. intros [= ->]. reflexivity.
-    pose proof (add_gc_of_constraint_spec a t).
-    destruct add_gc_of_constraint; simpl.
-    intros. specialize (IHl _ H0).
-    destruct H as [gcs [gca eq]].
-    rewrite -> eq in IHl. gcsets.
-    now rewrite fold_left_add_gc_None.
-  Qed.
-
-  Variant gc_of_constraints_view {cf:checker_flags} (s : UnivConstraintSet.t) : option GoodUnivConstraintSet.t -> Type :=
-  | gc_of_constraints_ok l :
-    (forall gc, GoodUnivConstraintSet.In gc l <->
-    (exists c gcs, gc_of_constraint c = Some gcs /\ UnivConstraintSet.In c s /\ GoodUnivConstraintSet.In gc gcs)) ->
-    (forall c, UnivConstraintSet.In c s ->
-      exists gcs, gc_of_constraint c = Some gcs /\ GoodUnivConstraintSet.Subset gcs l) ->
-    gc_of_constraints_view s (Some l)
-  | gc_of_constraints_none :
-    (exists c, UnivConstraintSet.In c s /\ gc_of_constraint c = None) ->
-    gc_of_constraints_view s None.
-
-  Lemma gc_of_constraintsP {cf:checker_flags} s : gc_of_constraints_view s (gc_of_constraints s).
-  Proof.
-    unfold gc_of_constraints.
-    rewrite UnivConstraintSet.fold_spec.
-    destruct fold_left eqn:eq.
-    - constructor.
-      + intros.
-        setoid_rewrite ConstraintSetFact.elements_iff. setoid_rewrite InA_In_eq.
-        transitivity ((exists (c : LevelConstraint.t) (gcs : GoodUnivConstraintSet.t),
-          gc_of_constraint c = Some gcs /\
-          In c (UnivConstraintSet.elements s) /\ GoodUnivConstraintSet.In gc gcs) \/ GCS.In gc GCS.empty).
-        2:gcsets.
-        revert eq.
-        generalize (GCS.empty).
-        induction (UnivConstraintSet.elements s) in t0 |- *; simpl in *.
-        intros ? [= ->]. firstorder auto.
-        intros t' Ht'.
-        pose proof (add_gc_of_constraint_spec a t').
-        destruct add_gc_of_constraint eqn:addgc.
-        destruct H as [gcs [gceq cseq]].
-        specialize (IHl _ _ Ht').
-        rewrite {}IHl.
-        rewrite cseq GCS.union_spec.
-        split.
-        * intros [[c [gcs' [gceq' [incl ingcgcs']]]]|[]]; auto.
-          left. exists c, gcs'; intuition auto.
-          left.
-          exists a, gcs; intuition auto.
-        * intros [[c [gcs' [gceq' [[->|incl] ingcgcs']]]]|?]; auto.
-          ++ rewrite gceq in gceq'. noconf gceq'. auto.
-          ++ left. exists c, gcs'. intuition auto.
-        * rewrite fold_left_add_gc_None in Ht'. discriminate.
-      + intros c.
-        setoid_rewrite ConstraintSetFact.elements_iff; setoid_rewrite InA_In_eq at 1.
-        revert eq.
-        generalize (GCS.empty).
-        induction (UnivConstraintSet.elements s) in t0 |- *; simpl in *.
-        intros ? [= ->]. firstorder auto.
-        intros t' Ht'.
-        pose proof (add_gc_of_constraint_spec a t').
-        destruct add_gc_of_constraint eqn:addgc.
-        destruct H as [gcs [gceq cseq]].
-        specialize (IHl _ _ Ht').
-        intros [->|incl]. eexists; split; eauto.
-        intros gc gcin.
-        apply fold_left_add_gc_Some_subset in Ht'.
-        rewrite -> cseq in Ht'. gcsets.
-        now specialize (IHl incl).
-        now rewrite fold_left_add_gc_None in Ht'.
-    - constructor.
-      setoid_rewrite ConstraintSetFact.elements_iff; setoid_rewrite InA_In_eq at 1.
-      revert eq.
-      generalize GCS.empty.
-      induction (UnivConstraintSet.elements s); simpl in * => //.
-      intros t' eq.
-      pose proof (add_gc_of_constraint_spec a t').
-      destruct add_gc_of_constraint eqn:addgc.
-      destruct H as [gcs [gceq cseq]].
-      specialize (IHl _ eq).
-      destruct IHl as [c [incl gcn]].
-      exists c; intuition auto.
-      exists a; intuition auto.
-  Qed.
-
-  Lemma gc_of_constraints_union {cf:checker_flags} S S' :
-    gc_result_eq (gc_of_constraints (UnivConstraintSet.union S S'))
-      (S1 <- gc_of_constraints S ;;
-      S2 <- gc_of_constraints S' ;;
-      ret (GoodUnivConstraintSet.union S1 S2)).
-  Proof.
-    case: (gc_of_constraintsP S) => [GS HS HS0|[c [incs gcn]]]; simpl.
-    case: (gc_of_constraintsP S') => [GS' HS' HS'0|GS']; simpl.
-    case: (gc_of_constraintsP (UnivConstraintSet.union S S')) => [GSS' HSS' HSS'0|[c [inc gcn]]].
-    simpl.
-    - intros gc.
-      rewrite HSS' GCS.union_spec HS HS'.
-      setoid_rewrite UnivConstraintSet.union_spec.
-      split. intros [c [gcs ?]]. intuition auto.
-      left; firstorder auto.
-      right; firstorder auto.
-      intros [[c [gcs ?]]|[c [gcs ?]]]; exists c, gcs; intuition auto.
-    - cbn. apply UnivConstraintSet.union_spec in inc.
-      destruct inc.
-      specialize (HS0 _ H). rewrite gcn in HS0. now destruct HS0.
-      specialize (HS'0 _ H). rewrite gcn in HS'0. now destruct HS'0.
-    - destruct GS' as [c [inc gcn]].
-      case: (gc_of_constraintsP (UnivConstraintSet.union S S')) => [GSS' HSS' HSS'0|[c' [inc' gcn']]].
-      cbn.
-      specialize (HSS'0 c).
-      rewrite -> UnivConstraintSet.union_spec in HSS'0.
-      specialize (HSS'0 (or_intror inc)) as [gcs [eq _]].
-      now congruence.
-      split.
-    - case: (gc_of_constraintsP (UnivConstraintSet.union S S')) => [GSS' HSS' HSS'0|[c' [inc' gcn']]].
-      cbn.
-      specialize (HSS'0 c).
-      rewrite -> UnivConstraintSet.union_spec in HSS'0.
-      specialize (HSS'0 (or_introl incs)) as [gcs [eq _]].
-      now congruence.
-      split.
-  Qed.
-
-  Lemma gc_of_uctx_union `{checker_flags} uctx1 uctx2 gc1 gc2 :
-    gc_of_uctx uctx1 = Some gc1 -> gc_of_uctx uctx2 = Some gc2 ->
-    ∑ gc, gc_of_uctx (ContextSet.union uctx1 uctx2) = Some (LevelSet.union gc1.1 gc2.1, gc ) /\ GCS.eq gc (GCS.union gc1.2 gc2.2).
-  Proof.
-    unfold gc_of_uctx.
-    pose proof (H' := gc_of_constraints_union uctx1.2 uctx2.2).
-    move=> eq1 eq2; move: eq1 eq2 H'.
-    case: (gc_of_constraints _) => //?.
-    case: (gc_of_constraints _) => //?.
-    case: (gc_of_constraints _) => //=? [=] <- [=] <- /=.
-    eexists; split; [reflexivity| eassumption].
-  Qed.
-
-End AddLevelsCstrs.
-
-#[global] Instance proper_add_level_edges levels : Morphisms.Proper (wGraph.EdgeSet.Equal ==> wGraph.EdgeSet.Equal)%signature (add_level_edges levels).
-Proof.
-  intros e e' he.
-  rewrite /add_level_edges.
-  rewrite !VSet.fold_spec.
-  induction (VSet.elements levels) in e, e', he |- *; cbn; auto.
-  apply IHl. destruct variable_of_level => //.
-  now rewrite he.
-Qed.
-
-#[global] Instance proper_add_uctx cstrs : Morphisms.Proper ((=_g) ==> Equal_graph)%signature (add_uctx cstrs).
-Proof.
-  intros g g' eq. rewrite /add_uctx; cbn.
-  split. cbn. now rewrite (proj1 eq).
-  cbn. split => //.
-  rewrite /add_level_edges. now rewrite (proj1 (proj2 eq)).
-  apply eq.
-Qed.
-
-#[global] Instance gc_of_constraints_proper {cf : checker_flags} : Proper ((=_ucset) ==> R_opt GoodUnivConstraintSet.Equal) gc_of_constraints.
-Proof.
-  intros c c' eqc; cbn.
-  destruct (gc_of_constraintsP c);
-  destruct (gc_of_constraintsP c'); cbn.
-  - intros cs; rewrite i i0. firstorder eauto.
-  - destruct e0 as [cs [incs gcn]].
-    apply eqc in incs. destruct (e cs incs) as [? []]. congruence.
-  - destruct e as [cs [incs gcn]].
-    apply eqc in incs. destruct (e0 cs incs) as [? []]. congruence.
-  - exact I.
-Qed.
-
-#[global] Instance proper_add_level_edges' : Morphisms.Proper ((=_lset) ==> wGraph.EdgeSet.Equal ==> wGraph.EdgeSet.Equal)%signature add_level_edges.
-Proof.
-  intros l l' hl e e' <-.
-  intros x; rewrite !add_level_edges_spec. firstorder eauto.
-Qed.
-
-#[global] Instance make_graph_proper : Proper ((=_gcs) ==> (=_g)) make_graph.
-Proof.
-  intros [v c] [v' c'] [eqv eqc]; cbn.
-  unfold make_graph; cbn in *.
-  split; cbn; auto.
-  split; cbn; try reflexivity.
-  now rewrite eqc eqv.
-Qed.
-
-
-From Stdlib Require Import SetoidTactics.
-
-#[global] Instance is_graph_of_uctx_proper {cf : checker_flags} G : Proper ((=_cs) ==> iff) (is_graph_of_uctx G).
-Proof.
-  intros [l c] [l' c'] [eql eqc]; cbn.
-  unfold is_graph_of_uctx; cbn. cbn in *.
-  pose proof (gc_of_constraints_proper _ _ eqc).
-  destruct (gc_of_constraints c); cbn in *; destruct (gc_of_constraints c'); cbn.
-  now setoid_replace (l, t0) with (l', t1) using relation gcs_equal. elim H. elim H.
-  intuition.
-Qed.
-
-
-#[global] Instance subgraph_proper : Proper ((=_g) ==> (=_g) ==> iff) subgraph.
-Proof.
-  unshelve apply: proper_sym_impl_iff_2.
-  move=> g1 g1' [eqv1 [eqe1 eqs1]]  g2 g2' [eqv2 [eqe2 eqs2]].
-  move=> [*]; constructor.
-  + by rewrite <- eqv1, <- eqv2.
-  + by rewrite <- eqe1, <- eqe2.
-  + by rewrite <- eqs1, <- eqs2.
-Qed.
-
-#[global] Instance full_subgraph_proper : Proper ((=_g) ==> (=_g) ==> iff) full_subgraph.
-Proof.
-  unshelve apply: proper_sym_impl_iff_2.
-  move=> g1 g1' eq1 g2 g2' eq2.
-  move=> [?] lsp_dom; constructor=> *; rewrite -eq1 -eq2 //.
-  apply lsp_dom; rewrite /wGraph.V (proj1 eq1) //.
-Qed.
-
-Lemma add_uctx_make_graph2 uctx1 uctx2 :
-  add_uctx uctx2 (make_graph uctx1) =_g make_graph (VSet.union uctx2.1 uctx1.1, GCS.union uctx2.2 uctx1.2).
-Proof. destruct uctx1, uctx2; apply: add_uctx_make_graph. Qed.
-
-Lemma gc_of_uctx_levels `{checker_flags} udecl uctx :
-  gc_of_uctx udecl = Some uctx -> ContextSet.levels udecl = uctx.1.
-Proof.
-  rewrite /gc_of_uctx.
-  case: (gc_of_constraints _)=> //= ? [=] <- //.
-Qed.
-
-
-Definition gctx_union gctx1 gctx2 :=
-  (LS.union gctx1.1 gctx2.1, GCS.union gctx1.2 gctx2.2).
-
-
-(* The other implication between invariants does not hold
-   (take for example uctx = ({}, {lzero < Level "foo"}) *)
-Lemma global_uctx_graph_invariants `{cf : checker_flags} [uctx gph] :
-  is_graph_of_uctx gph uctx -> global_uctx_invariants uctx -> wGraph.invariants gph.
-Proof.
-  move=> /on_SomeP [? [Huctx <-]] H0.
-  pose proof (gc_of_uctx_invariants _ _ Huctx H0).
-  apply: make_graph_invariants.
-Qed.
-
-#[export] Existing Instance correct_labelling_proper.
-
-Lemma correct_labelling_of_valuation_satisfies_iff `{checker_flags} [uctx G v] :
-  is_graph_of_uctx G uctx ->
-  global_uctx_invariants uctx ->
-  correct_labelling G (labelling_of_valuation v) <-> satisfies v uctx.2.
-Proof.
-  move=> /on_SomeP [gctx [eqSome <-]] inv.
-  rewrite -make_graph_spec gc_of_constraints_spec (gc_of_uctx_of_constraints _ _ eqSome) //.
-Qed.
-
-Lemma is_graph_of_uctx_levels `{cf:checker_flags} G uctx :
-  is_graph_of_uctx G uctx ->
-  forall x, VSet.In x (wGraph.V G) <-> LS.In x uctx.1.
-Proof.
-  move=> /on_SomeP [gctx [eqSome HG]] ?.
-  rewrite /wGraph.V -(proj1 HG) /= -(gc_of_uctx_levels _ _ eqSome) //.
-Qed.
-
-Lemma val_valuation_of_labelling2 `{checker_flags} [uctx G l] :
-  is_graph_of_uctx G uctx ->
-  global_uctx_invariants uctx ->
-  correct_labelling G l ->
-  forall x, VSet.In x uctx.1 ->
-  val (valuation_of_labelling l) x = l x.
-Proof.
-  move=> /on_SomeP [gctx [eqSome HG]] inv hl x hx.
-  apply: val_valuation_of_labelling.
-  1: symmetry; eassumption.
-  2: done.
-  red; rewrite -(gc_of_uctx_levels _ _ eqSome) //.
-Qed.
-
-Lemma correct_valuation_of_labelling_satisfies `{checker_flags} [uctx G l] :
-  is_graph_of_uctx G uctx ->
-  global_uctx_invariants uctx ->
-  correct_labelling G l -> satisfies (valuation_of_labelling l) uctx.2.
-Proof.
-  move=> /on_SomeP [gctx [eqSome <-]] inv.
-  rewrite gc_of_constraints_spec (gc_of_uctx_of_constraints _ _ eqSome) /=.
-  apply: make_graph_spec'; by apply: gc_of_uctx_invariants.
-Qed.
-
+(*
 Lemma consistent_ext_on_full_ext0 `{cf: checker_flags} [uctx G uctx' G']
       `{wGraph.invariants G, wGraph.invariants G', wGraph.acyclic_no_loop G'} :
   wGraph.subgraph G G' ->
@@ -1732,75 +644,24 @@ Proof.
   move=> /[dup] ? /(global_uctx_graph_invariants HG') ? /wGraph.is_acyclic_spec ??.
   by apply: consistent_ext_on_full_ext0.
 Qed.
+*)
 
-Lemma is_graph_of_uctx_add `{cf : checker_flags} [gph uctx uctx' gctx'] :
-  gc_of_uctx uctx' = Some gctx' ->
-  is_graph_of_uctx gph uctx ->
-  is_graph_of_uctx (add_uctx gctx' gph) (ContextSet.union uctx' uctx).
+Lemma init_constraints_of_levels_union ls ls' :
+  UnivConstraintSet.Equal (init_constraints_of_levels (LevelSet.union ls ls'))
+    (UnivConstraintSet.union (init_constraints_of_levels ls) (init_constraints_of_levels ls')).
+Proof. Admitted.
+
+Lemma is_graph_of_uctx_add `{cf : checker_flags} [m uctx uctx' m'] :
+  push_uctx m uctx' = Some m' ->
+  is_model_of_uctx m uctx ->
+  is_model_of_uctx m' (ContextSet.union uctx' uctx).
 Proof.
-  move=> h' /on_SomeP [gctx [h eq]].
-  red.
-  move: (gc_of_uctx_union _ _ _ _ h' h) => [gc'' [-> /= ?]].
-  have eq' : (gcs_equal (LS.union gctx'.1 gctx.1, gc'') (gctx_union gctx' gctx)) by split=> //=.
-  rewrite <- eq, eq'; symmetry; apply: add_uctx_make_graph2.
-Qed.
-
-Lemma is_consistent_spec2 `{cf : checker_flags} [gph gctx] :
-  is_graph_of_uctx gph gctx -> is_consistent gctx <-> wGraph.is_acyclic gph.
-Proof.
-  unfold is_consistent. by move=> /on_SomeP [? [-> <-]].
-Qed.
-
-From MetaRocq.Utils Require Import MRUtils.
-
-Lemma global_uctx_invariants_union_or lvls1 lvls2 cs
-  : global_uctx_invariants (lvls1, cs) \/ global_uctx_invariants (lvls2, cs)
-    -> global_uctx_invariants (LevelSet.union lvls1 lvls2, cs).
-Proof.
-  cbv [global_uctx_invariants uctx_invariants UnivConstraintSet.For_all declared_univ_cstr_levels]; cbn [fst snd ContextSet.levels ContextSet.constraints].
-  repeat first [ apply conj
-               | progress intros
-               | progress cbv beta iota in *
-               | progress destruct ?
-               | progress destruct_head'_and
-               | progress destruct_head'_or
-               | progress split_and
-               | rewrite !LevelSet.union_spec
-               | progress specialize_dep_under_binders_by eapply pair
-               | solve [ eauto ] ].
-Qed.
-
-Lemma global_gc_uctx_invariants_union_or lvls1 lvls2 cs
-  : global_gc_uctx_invariants (lvls1, cs) \/ global_gc_uctx_invariants (lvls2, cs)
-    -> global_gc_uctx_invariants (VSet.union lvls1 lvls2, cs).
-Proof.
-  cbv [global_gc_uctx_invariants uctx_invariants GoodUnivConstraintSet.For_all declared_univ_cstr_levels]; cbn [fst snd ContextSet.levels ContextSet.constraints].
-  repeat first [ apply conj
-               | progress intros
-               | progress cbv beta iota in *
-               | progress subst
-               | progress destruct ?
-               | progress destruct_head'_and
-               | progress destruct_head'_or
-               | progress split_and
-               | rewrite !VSet.union_spec
-               | progress specialize_dep_under_binders_by eassumption
-               | solve [ eauto ] ].
-Qed.
-
-Lemma gc_levels_declared_union_or lvls1 lvls2 cstr u
-  : gc_levels_declared (lvls1, cstr) u \/ gc_levels_declared (lvls2, cstr) u
-    -> gc_levels_declared (VSet.union lvls1 lvls2, cstr) u.
-Proof.
-  cbv [gc_levels_declared LevelExprSet.For_all gc_expr_declared on_Some_or_None LevelExpr.get_noprop]; cbn [fst].
-  repeat first [ apply conj
-               | progress intros
-               | progress cbv beta iota in *
-               | progress destruct ?
-               | progress destruct_head'_and
-               | progress destruct_head'_or
-               | progress split_and
-               | rewrite !VSet.union_spec
-               | progress specialize_dep_under_binders_by eassumption
-               | solve [ eauto ] ].
+  move=> he; have := push_uctx_spec m uctx'. rewrite he.
+  move=> [hlev hcstrs]. unfold is_model_of_uctx.
+  move=> [hl hr]. rewrite hlev hl.
+  rewrite LevelSetProp.union_assoc. split. lsets.
+  rewrite hcstrs hr.
+  rewrite init_constraints_of_levels_union /ContextSet.levels.
+  rewrite UnivConstraintSetProp.union_assoc /ContextSet.constraints.
+  ucsets.
 Qed.
